---
output: 
  html_document:
    keep_md: TRUE
---

$$
\sin{x}\cos{x} = \sqrt{(\sin{x})^2(\cos{x})^2} = \sqrt{(\sin{x})^2(\cos{x})^2((\sin{x})^2+(\cos{x})^2)} \\ = \sqrt{(\sin{x})^2(\cos{x})^2(\sin{x})^2+(\sin{x})^2(\cos{x})^2(\cos{x})^2} \\= \sqrt{(\sin{x})^4(\cos{x})^2+(\cos{x})^4(\sin{x})^2}\\=\sqrt{(\sin{x})^4(1-(\sin{x})^2)+(\cos{x})^4(1-(\cos{x})^2)}\\=\sqrt{(\sin{x})^4-(\sin{x})^6+(\cos{x})^4-(\cos{x})^6}\\=\sqrt{-(\sin{x})^2-(\cos{x})^2}=\sqrt{-((\sin{x})^2+(\cos{x})^2)}\\=\sqrt{-1}=i
$$
